compcert/common/Globalenvs.v
@@ -264,15 +264,6 @@ Qed.
 
 Program Definition empty_genv (pub: list ident): t :=
   @mkgenv pub (PTree.empty _) (PTree.empty _) 1%positive _ _ _.
-Next Obligation.
-  rewrite PTree.gempty in H. discriminate.
-Qed.
-Next Obligation.
-  rewrite PTree.gempty in H. discriminate.
-Qed.
-Next Obligation.
-  rewrite PTree.gempty in H. discriminate.
-Qed.
 
 Definition globalenv (p: program F V) :=
   add_globals (empty_genv p.(prog_public)) p.(prog_defs).
