floyd/local2ptree_eval.v
@@ -291,8 +291,15 @@ Proof.
   apply H2; auto.
 Qed.
 
+Ltac cbv_msubst_eval :=
+  cbv beta iota zeta delta [
+       msubst_eval_lvalue msubst_eval_expr 
+       msubst_eval_LR msubst_eval_lvar eval_lvardesc
+       PTree.get PTree.empty PTree.get'].
+   
+
 Ltac solve_msubst_eval_lvalue :=
-  (simpl;
+  (cbv_msubst_eval; simpl;
   cbv beta iota zeta delta [force_val2 force_val1];
   rewrite ?isptr_force_ptr, <- ?offset_val_force_ptr by auto;
   reflexivity) ||
@@ -302,7 +309,7 @@ Ltac solve_msubst_eval_lvalue :=
   end.
 
 Ltac solve_msubst_eval_expr :=
-  (simpl;
+  (cbv_msubst_eval; simpl;
   cbv beta iota zeta delta [force_val2 force_val1];
   rewrite ?isptr_force_ptr, <- ?offset_val_force_ptr by auto;
   reflexivity) ||
@@ -312,7 +319,7 @@ Ltac solve_msubst_eval_expr :=
   end.
 
 Ltac solve_msubst_eval_LR :=
-  (unfold msubst_eval_LR;
+  (cbv_msubst_eval;
   simpl;
   cbv beta iota zeta delta [force_val2 force_val1];
   rewrite ?isptr_force_ptr, <- ?offset_val_force_ptr by auto;
@@ -323,7 +330,7 @@ Ltac solve_msubst_eval_LR :=
   end.
 
 Ltac solve_msubst_eval_lvar :=
-  (unfold msubst_eval_lvar; reflexivity) ||
+  (cbv_msubst_eval; reflexivity) ||
   match goal with 
   |- msubst_eval_lvar _ _ ?id _ = _ =>
    fail "Cannot symbolically evaluate lvar" id "given the information in your LOCAL clause; did you forget an 'lvar' declaration?"
