progs/conclib.v
@@ -1863,7 +1863,7 @@ Proof.
   - unfold make_tycontext_g.
     revert dependent G2; revert dependent V2; revert V; induction G; simpl.
     + induction V; simpl; intros.
-      * rewrite PTree.gempty; simpl; auto.
+      *  auto.
       * rewrite incl_cons_iff in HV; destruct HV.
         rewrite PTree.gsspec.
         destruct (peq id (fst a)); eauto; subst; simpl.
@@ -1878,7 +1878,7 @@ Proof.
       apply lookup_distinct; auto.
   - unfold make_tycontext_s.
     revert dependent G2; induction G; simpl; intros.
-    + rewrite PTree.gempty; simpl; auto.
+    +  auto.
     + destruct a; simpl. hnf.
       rewrite incl_cons_iff in HG; destruct HG.
       rewrite PTree.gsspec.
